Proof

ArchSemArm/ArmSeqAxOpEq.v
@@ -1,6 +1,6 @@
 Require Import ArmSeqModel UMSeqArm.
 Require Import ArmInst.
-From ASCommon Require Import Exec FMon Common Options.
+From ASCommon Require Import Exec FMon Common Options GRel StateT.
 
 Import CDestrUnfoldElemOf.
 #[local] Existing Instance Exec.unfold.
@@ -23,6 +23,16 @@ Proof.
   set_unfold. autorewrite with pair. naive_solver.
 Qed.
 
+Instance Exec_to_state_result_list {St E A} r (e : Exec.res (St * E) (St * A)) P Q:
+  (∀ st v, SetUnfoldElemOf (st, v) e (P st v)) →
+  (∀ st v, SetUnfoldElemOf (st, v) e.(Exec.errors) (Q st v)) →
+  SetUnfoldElemOf r (Exec.to_state_result_list e)
+    (match r with
+    | Ok st => ∃ v, P st v
+    | Error st => ∃ v, Q st v
+    end) | 999 .
+Proof. tcclean. destruct r; set_solver. Qed.
+
 Lemma finterp_inv_induct `{Effect Eff} {St E A}
   (handler : fHandler Eff (Exec.t St E)) (mon : fMon Eff A)
   (I : result St St → Prop) (initSt : St)
@@ -32,33 +42,8 @@ Lemma finterp_inv_induct `{Effect Eff} {St E A}
 Proof.
   intros Hinit Hstep.
   induction mon as [|? ? IH] in initSt, Hinit |- *;
-    cdestruct |- *** as st' Hst'.
-  destruct st'; cdestruct Hst' #CDestrSplitGoal.
-  - (* Success *)
-    eapply (IH x1 x0).
-    2: { set_solver. }
-    eapply (Hstep initSt call).
-    2: { set_solver. }
-    assumption.
-  - (* Error in handling of call *)
-    eapply (Hstep initSt call).
-    2: set_solver.
-    assumption.
-  - (* Error in handling of continuation k *)
-    eapply (IH x1 x0).
-    2:set_solver.
-    eapply (Hstep initSt call).
-    2:set_solver.
-    assumption.
-Qed.
-
-Instance Exec_mcall_MChoice {St E A} st (e : Exec.res (St * E) (St * A)) P:
-  (∀ v, SetUnfoldElemOf (st, v) e.(Exec.errors) (P v)) →
-  SetUnfoldElemOf (Error st) (Exec.to_state_result_list e) (∃ v, P v).
-Proof.
-  tcclean.
-  unfold Exec.to_state_result_list.
-  set_unfold. autorewrite with pair. naive_solver.
+  cdestruct |- *** #CDestrMatch;
+  set_solver.
 Qed.
 
 Arguments Exec.to_state_result_list : simpl never.
@@ -73,13 +58,9 @@ Proof.
   intros Hinit HIpreserve st' Hst'.
   eapply finterp_inv_induct; [eassumption | | eassumption].
   clear initSt Hinit st' Hst'.
-  intros st [|[]] Hst st' Hst'.
-  - cbn in Hst'. naive_solver.
-  - destruct st'.
-    + cdestruct Hst'.
-      unfold Exec.Results in H0.
-      cdestruct val |- ***.
-    + cdestruct Hst'.
+  cdestruct |- *** as st eff Hst st' v Hst' #CDestrMatch #CDestrSplitGoal;
+  try destruct eff;
+  set_solver.
 Qed.
 
 (* TODO:
@@ -111,21 +92,95 @@ Fixpoint trace_find (P : FMon.fEvent outcome → Prop) `{∀ x, Decision (P x)}
   | [] => None
   end.
 
+Lemma trace_find_app (P : FMon.fEvent outcome → Prop) `{∀ x, Decision (P x)}
+  (l l' : list (iTrace ()))
+  : trace_find P (l ++ l') = if trace_find P l is Some ev then Some ev else trace_find P l'.
+Proof. induction l; cdestruct |- *** #CDestrMatch. Qed.
+
+Definition trace_rev (itrs : list (iTrace ())) : list (iTrace ()) :=
+  rev (map (set fst (@rev (FMon.fEvent outcome))) itrs).
+
+Fixpoint find_last_aux {A} (P : A → Prop) `{∀ x, Decision (P x)} (acc : option A) (l : list A) : option A :=
+  if l is a :: ar
+  then find_last_aux P (if decide (P a) then Some a else acc) ar
+  else acc.
+
+Definition find_last {A} (P : A → Prop) `{∀ x, Decision (P x)} : list A → option A :=
+  find_last_aux P None.
+
+Lemma find_app {A} (P : A → bool) `{∀ x, Decision (P x)} (l l' : list A)
+  : find P (l ++ l') = if find P l is Some a then Some a else find P l'.
+Proof. induction l; cdestruct |- *** #CDestrMatch. Qed.
+
+Lemma find_rev_find_last {A} (P : A → Prop) `{∀ x, Decision (P x)} (l : list A)
+  : find (λ x, bool_decide (P x)) (rev l) = find_last P l.
+Proof.
+  unfold find_last.
+  enough (∀ o, (if find (λ x : A, bool_decide (P x)) (rev l) is Some a then Some a else o) = find_last_aux P o l)
+  as <- by cdestruct |- *** #CDestrMatch.
+  induction l; first done; cdestruct |- ***.
+  rewrite <- IHl.
+  rewrite find_app; cdestruct |- *** #CDestrMatch; tc_solve.
+Qed.
+
+Fixpoint trace_find_last_aux (P : FMon.fEvent outcome → Prop) `{∀ x, Decision (P x)}
+  (acc : option (FMon.fEvent outcome)) (itrs : list (iTrace ())) : option (FMon.fEvent outcome) :=
+  match itrs with
+  | ((itr, trend) :: itrr) =>
+    trace_find_last_aux P (if find_last P itr is Some ev then Some ev else acc) itrr
+  | [] => acc
+  end.
+
+Definition trace_find_last (P : FMon.fEvent outcome → Prop) `{∀ x, Decision (P x)}
+  : list (iTrace ()) → option (FMon.fEvent outcome) :=
+  trace_find_last_aux P None.
+
+Lemma find_trace_rev_find_trace_list (P : FMon.fEvent outcome → Prop) `{∀ x, Decision (P x)}
+  (acc : option (FMon.fEvent outcome)) (itrs : list (iTrace ()))
+  : trace_find P (trace_rev itrs) = trace_find_last P itrs.
+Proof.
+  unfold trace_find_last.
+  enough (∀ o, (if trace_find P (trace_rev itrs) is Some ev then Some ev else o)
+                = trace_find_last_aux P o itrs)
+  as <- by cdestruct |- *** #CDestrMatch.
+  unfold trace_rev.
+  induction itrs as [|[]]; cdestruct |- ***.
+  rewrite trace_find_app.
+  cbn.
+  rewrite <- find_rev_find_last.
+  setoid_rewrite <- IHitrs.
+  cdestruct |- *** #CDestrMatch.
+Qed.
+
 Lemma trace_find_cons (P : FMon.fEvent outcome → Prop) `{∀ x, Decision (P x)}
     (itrs : list (iTrace ())) (x : FMon.fEvent outcome)
-  : trace_find P (set fst (cons x) (hd FTNothing itrs) :: tail itrs) =
+  : trace_find P (trace_cons x itrs) =
     if decide (P x)
     then Some x
     else trace_find P itrs.
 Proof.
-  (* TODO TP: Fix cdestruct for contradiction and i *)
-  destruct itrs. all: cdestruct |- *** #CDestrMatch #CDestrEqOpt.
-  all: cdestruct i |- *** #CDestrEqOpt.
+  destruct itrs as [|[]].
+  all: cdestruct |- *** #CDestrMatch #CDestrEqOpt.
+Qed.
+
+#[global] Instance elem_of_trace : ElemOf (fEvent outcome) (list (iTrace ())) :=
+  λ ev itrs, ev ∈ (mjoin (fst <$> itrs)).
+
+#[export] Instance unfold_elem_of_trace_cons ev ev' itrs P :
+  SetUnfoldElemOf ev itrs P →
+  SetUnfoldElemOf ev (trace_cons ev' itrs) (ev = ev' ∨ P).
+Proof.
+  tcclean.
+  unfold elem_of, elem_of_trace.
+  unfold trace_cons.
+  destruct itrs as [|[]].
+  all: set_solver.
 Qed.
 
 Arguments trace_find : simpl never.
 
-Print Coercions.
+Section Proof.
+Search bv_modulus.
 Context (regs_whitelist : option (gset reg)) (fuel : nat) (isem : iMon ()).
 
 Notation seqmon := (Exec.t seq_state string).
@@ -134,6 +189,12 @@ Notation initss := {| initSt := initSt; regs := ∅; mem := ∅; itrs := [] |}.
 Definition seqmon_pe (st : seq_state) : Candidate.pre Candidate.NMS 1 :=
   Candidate.make_pre _ st.(initSt) [# st.(itrs)].
 
+Definition result_same_type_proj {T} (r : result T T) :=
+  match r with
+  | Ok t => t
+  | Error t => t
+  end.
+
 Definition op_mem_wf (str : result seq_state seq_state) : Prop :=
   match str with
   | Ok st =>
@@ -141,10 +202,10 @@ Definition op_mem_wf (str : result seq_state seq_state) : Prop :=
       st.(mem) !! pa = Some v
     ↔ ∃ ev,
         trace_find
-          (is_mem_writeP (λ size wr, pa_in_range wr.(WriteReq.pa) (Z.to_N (Z.min (Z.of_N size) (bv_modulus 52))) pa))
+          (is_mem_writeP (λ size wr, pa_in_range wr.(WriteReq.pa) size pa))
           st.(itrs)
         = Some ev
-    ∧ ∃ offset, (0 ≤ Z.of_N offset < bv_modulus 52)%Z ∧
+    ∧ ∃ offset,
         ev |> is_mem_writeP
           (λ size wr,
             pa_addN wr.(WriteReq.pa) offset = pa
@@ -153,18 +214,11 @@ Definition op_mem_wf (str : result seq_state seq_state) : Prop :=
   | Error _ => False
   end.
 
-
-Definition result_same_type_proj {T} (r : result T T) :=
-  match r with
-  | Ok t => t
-  | Error t => t
-  end.
-
 Lemma length_bv_to_bytes n m (v : bv n) :
   length (bv_to_bytes m v) = N.to_nat (div_round_up n m).
 Proof.
   unfold bv_to_bytes.
-  rewrite bv_to_little_endian_length.
+  rewrite length_bv_to_little_endian.
   2: lia.
   rewrite <- Z_N_nat.
   now rewrite N2Z.id.
@@ -215,65 +269,171 @@ Proof.
   eapply IHbytes, H.
 Qed.
 
+Context (max_size : N) {max_size_upper_limit : (max_size < Z.to_N (bv_modulus 52))%N}.
+
+Definition tr_wf (str : result seq_state seq_state) : Prop :=
+  match str with
+  | Ok st =>
+    (∀ ev ∈ st.(itrs), is_mem_write ev → is_mem_writeP (λ size _, (size < max_size)%N) ev)
+  | Error _ => False
+  end.
+
 Lemma op_reads st :
+  tr_wf (Ok st) →
   op_mem_wf (Ok st) →
-  ∀ str ∈ (Exec.to_state_result_list $ FMon.cinterp (sequential_model_outcome_logged regs_whitelist) isem st),
-  (λ str, is_Ok str → op_mem_wf str) str.
+  ∀ str ∈ (Exec.to_state_result_list $ FMon.cinterp (sequential_model_outcome_logged regs_whitelist (Z.to_N (bv_modulus 52))) isem st),
+  (λ str, is_Ok str → tr_wf str → op_mem_wf str) str.
 Proof.
-  intro.
-  eapply cinterp_inv_induct; first easy; clear.
+  intros Htr Hmem.
+  eapply cinterp_inv_induct; first easy; clear Htr Hmem st.
   cdestruct |- *** as st call H_st st' H_st' pa.
-  unfold Exec.to_state_result_list in *.
-  cdestruct H_st' as r H_st' v #CDestrSplitGoal.
+  cdestruct H_st' as r H_st' Hsize v #CDestrSplitGoal.
+  (* Case split: Is newest event a memory write? *)
   destruct (decide (is_mem_write (call &→ r))).
-  2: {
+  2: { (* Not mem write: no changes to mem map and remaining trace is still wf *)
     destruct call.
     all: do 7 deintro.
     all: cdestruct |- *** #CDestrMatch.
-    all: rewrite trace_find_cons.
+    all: rewrite trace_find_cons in *.
     all: cdestruct |- *** #CDestrMatch.
     all: try easy.
     all: eapply H_st.
     all: cdestruct |- ***.
+    all: set_unfold in Hsize.
+    all: naive_solver.
   }
+  (* mem write: memory map at pa is exactly written byte and otherwise unchanged *)
   destruct call; try easy.
-  do 9 deintro.
+  do 6 deintro.
   cdestruct |- *** #CDestrMatch.
   rewrite trace_find_cons.
-  inversion H0.
+  inversion H1.
   do 11 deintro;
-  cdestruct |- *** as ?? st' Hst' pa ?? #CDestrMatch.
+  cdestruct |- *** as st' ? Hst' Hsize pa ?? #CDestrMatch.
   2: {
     assert (mem st' !! pa = mem st !! pa) as ->.
     {
       eapply pa_not_in_range_write; eauto.
       rewrite length_bv_to_bytes.
       f_equal.
-      admit.
+      now eapply div_round_up_divisible.
     }
-    erewrite write_mem_seq_state_itrs; last eauto.
-    eapply H_st.
+    erewrite write_mem_seq_state_itrs in Hsize |- *; eauto.
+    eapply H_st;
     cdestruct |- ***.
+    set_solver.
     }
   apply pa_in_range_spec in p.
   cdestruct p as offset H_pa H_offset.
-  enough (mem st' !! pa = Some (bv_get_byte 8 offset (WriteReq.value wr))) as ->.
-  {
-    cdestruct |- *** #CDestrSplitGoal.
-    - eexists; cdestruct |- *** #CDestrSplitGoal; eauto.
-      eexists offset.
-      cdestruct |- *** #CDestrSplitGoal; lia.
-    - inversion H1; subst.
-      deintro; cdestruct |- ***.
-      f_equal; last naive_solver.
-      subst.
-      destruct x1, pa0; cbn in *.
-      unfold pa_addN, pa_addZ in H2; cbv in H2.
-      cdestruct H2.
-      eapply bv_add_Z_inj_l in H2.
-      1: deintro.
-      all: cdestruct |- *** #CDestrMatch; lia.
-  }
-  assert (offset < n)%N by lia.
-  eapply pa_offset_in_range_write; eauto.
+  assert (mem st' !! pa = Some (bv_get_byte 8 offset (WriteReq.value wr))) as ->
+  by (eapply pa_offset_in_range_write; eauto).
+  cdestruct |- *** #CDestrSplitGoal.
+  - eexists; cdestruct |- *** #CDestrSplitGoal; eauto.
+    eexists offset.
+    cdestruct |- *** #CDestrSplitGoal; lia.
+  - inversion H0; subst.
+    deintro; cdestruct |- ***.
+    f_equal; last naive_solver.
+    subst.
+    destruct x1; cbn in *.
+    unfold pa_addN, pa_addZ in H1; cbv in H1.
+    cdestruct H1.
+    assert (x0 < max_size)%N
+    by (set_unfold in Hsize; opose proof (Hsize _ (or_introl _) _); by eauto).
+    eapply bv_add_Z_inj_l in H1.
+    all: do 2 deintro; cdestruct |- *** #CDestrSplitGoal #CDestrMatch; lia.
 Admitted.
+
+Context {et : Candidate.exec_type}.
+
+Notation "( f <$>.)" := (fmap f) (only parsing) : stdpp_scope.
+
+Record cd_state := {
+  map_acc : gmap pa EID.t;
+  rf_acc : grel EID.t;
+  rrf_acc : grel EID.t;
+  co_acc : grel EID.t
+}.
+
+#[global] Instance eta_rf_state : Settable rf_state :=
+  settable! Build_rf_state <map_acc;rf_acc;rrf_acc;co_acc>.
+
+Fixpoint write_eids_to_pa_map (pas : list pa) (st : rf_state) : rf_state :=
+  if pas is pa :: par
+  then
+    st
+    |> setv (lookup pa ∘ map_acc) (Some st.(eid_acc))
+    |> write_eids_to_pa_map par
+  else st.
+
+Fixpoint read_to_rf_acc (pas : list pa) (st : rf_state) : rf_state :=
+  if pas is pa :: par
+  then
+    let reid := st.(eid_acc) in
+    let oweid := st.(map_acc) !! pa in
+    st
+    |> (if oweid is Some weid
+        then set rf_acc ({[((weid,reid))]} ∪.)
+        else id)
+    |> set (EID.byte ∘ eid_acc) (N.succ <$>.)
+    |> read_to_rf_acc par
+  else st.
+
+Definition construct_rf_fo_itr (itr : iTrace ()) : rf_state → rf_state :=
+  fold_left
+    (λ st ev,
+      match ev with
+      | MemWrite n wr &→ r =>
+        st
+        |> write_eids_to_pa_map
+           (if et is Candidate.NMS
+            then [wr.(WriteReq.pa)]
+            else pa_range wr.(WriteReq.pa) n)
+      | MemRead n rr &→ r =>
+        st
+        |> (if et is Candidate.NMS
+            then id
+            else setv (EID.byte ∘ eid_acc) (Some 0%N))
+        |> read_to_rf_acc (pa_range rr.(ReadReq.pa) n)
+      | _  => st
+      end
+      |> set (EID.ieid ∘ eid_acc) S
+      |> setv (EID.byte ∘ eid_acc) None)
+    itr.1.
+
+
+Definition construct_rf_for_pe '(Candidate.make_pre _ init events : Candidate.pre Candidate.NMS 1) : rf_state → rf_state :=
+  fold_left (B := (iTrace ()))
+    (λ st itr,
+      construct_rf_fo_itr itr st
+      |> set (EID.iid ∘ eid_acc) S
+      |> setv (EID.ieid ∘ eid_acc) 0)
+    (events !!! 0%fin).
+
+Lemma op_model_to_cd
+
+Theorem op_model_soundness max_mem_acc_size ax initSt:
+  Model.Res.weaker
+    ((Model.to_nc $ sequential_modelc regs_whitelist max_mem_acc_size fuel isem) 1 initSt)
+    (Ax.to_Modelnc (et := Candidate.NMS) isem ax 1 initSt).
+Proof.
+  cdestruct |- *** as Ax_no_err.
+  split.
+  - cdestruct |- *** as axfs H_axfs.
+    Transparent propset_bind propset_ret.
+    unfold propset_bind in *.
+    cdestruct axfs, H_axfs |- *** as [] m H_ofinst H_finst.
+    exists m.
+    destruct m; cbn in *.
+    2,3: unfold mfail , set_mfail in *; set_solver.
+    split.
+    1: done.
+    unfold mret, propset_ret in *.
+    cdestruct finSt, H_ofinst.
+    unfold elem_of, listset_elem_of in H_finst.
+    cdestruct H_finst.
+    destruct r; cbn in *.
+    2: done.
+Abort.
+
+End Proof.
